refactor proofs, first part

examples/riscv/incr/incr_propScript.sml
@@ -73,6 +73,8 @@ Definition bir_incr_pre_def:
     (BExp_Const (Imm64 x))
 End
 
+val bir_incr_pre = ``bir_incr_pre``;
+
 Definition bir_incr_post_def:
  bir_incr_post x : bir_exp_t =
   BExp_BinPred
@@ -131,24 +133,21 @@ End
 val birs_state_init_lbl = ``<|bpc_label := BL_Address (Imm64 0w); bpc_index := 0|>``;
 val birs_state_end_lbl = (snd o dest_eq o concl o EVAL) ``bir_block_pc (BL_Address (Imm64 4w))``;
 
-Definition bprecond_def:
-  bprecond = bir_incr_pre
-End
+val birs_state_ss = rewrites (type_rws ``:birs_state_t``);
 
-val bprecond = (fst o dest_eq o concl) bprecond_def;
-
+(*
 Definition bsysprecond_def:
-  bsysprecond x = FST (THE (birs_eval_exp (^bprecond x) (bir_senv_GEN_list incr_birenvtyl)))
+  bsysprecond x = FST (THE (birs_eval_exp (^bir_incr_pre x) (bir_senv_GEN_list incr_birenvtyl)))
 End
 
-Theorem bprecond_birs_eval_exp_thm = (computeLib.RESTR_EVAL_CONV [``birs_eval_exp``] THENC
+Theorem bir_incr_pre_birs_eval_exp_thm = (computeLib.RESTR_EVAL_CONV [``birs_eval_exp``] THENC
    birs_stepLib.birs_eval_exp_CONV)
-     ``birs_eval_exp (bprecond pre_x10) (bir_senv_GEN_list incr_birenvtyl)``
+     ``birs_eval_exp (bir_incr_pre pre_x10) (bir_senv_GEN_list incr_birenvtyl)``
 
 Theorem bsysprecond_thm =
- (REWRITE_CONV [bsysprecond_def, birs_eval_exp_ALT_thm, bprecond_birs_eval_exp_thm] THENC EVAL) ``bsysprecond pre_x10``
+ (REWRITE_CONV [bsysprecond_def, birs_eval_exp_ALT_thm, bir_incr_pre_birs_eval_exp_thm] THENC EVAL) ``bsysprecond pre_x10``
 
-Theorem bprecond_birs_eval_exp_thm2 = REWRITE_CONV [bprecond_birs_eval_exp_thm, GSYM bsysprecond_thm] ``birs_eval_exp (bprecond pre_x10) (bir_senv_GEN_list incr_birenvtyl)``
+Theorem bir_incr_pre_birs_eval_exp_thm2 = REWRITE_CONV [bir_incr_pre_birs_eval_exp_thm, GSYM bsysprecond_thm] ``birs_eval_exp (bir_incr_pre pre_x10) (bir_senv_GEN_list incr_birenvtyl)``
 
 val bsysprecond = (fst o dest_eq o concl o Q.SPEC `pre_x10`) bsysprecond_def;
 
@@ -158,120 +157,143 @@ val birs_state_init_pre = ``<|
   bsst_status   := BST_Running;
   bsst_pcond    := ^bsysprecond
 |>``;
+*)
 
-val birs_state_ss = rewrites (type_rws ``:birs_state_t``);
-val birs_state_init_pre_EQ_thm =
- REWRITE_RULE [] ((REWRITE_CONV [bsysprecond_thm] THENC
-  SIMP_CONV (std_ss++birs_state_ss++holBACore_ss) [] THENC
-  EVAL)
-  ``^((snd o dest_comb) sys_i) = ^birs_state_init_pre``);
 
-val incr_analysis_thm =
-  REWRITE_RULE [birs_state_init_pre_EQ_thm, GSYM bir_incr_prog_def] incr_symb_analysis_thm;
 
-Theorem incr_birenvtyl_EVAL_thm =
- (REWRITE_CONV [incr_birenvtyl_def,
-   bir_lifting_machinesTheory.riscv_bmr_vars_EVAL,
-   bir_lifting_machinesTheory.riscv_bmr_temp_vars_EVAL] THENC EVAL)
- ``incr_birenvtyl``
-
-val birs_state_thm = REWRITE_CONV [incr_birenvtyl_EVAL_thm] birs_state_init_pre;
-
-(* ------ *)
-
-(* now the transfer *)
-
-val bprog_tm = (fst o dest_eq o concl) bir_incr_prog_def;
-
-val birs_symb_symbols_f_sound_prog_thm =
-  (SPEC (inst [Type`:'observation_type` |-> Type.alpha] bprog_tm) bir_symb_soundTheory.birs_symb_symbols_f_sound_thm);
-
-val birs_prop_transfer_thm =
-  (MATCH_MP symb_prop_transferTheory.symb_prop_transfer_thm birs_symb_symbols_f_sound_prog_thm);
-
-Definition bprog_P_def:
-  bprog_P x ((SymbConcSt pc st status):(bir_programcounter_t, string, bir_val_t, bir_status_t) symb_concst_t) =
+(* TODO: MOVE AWAY !!!!! GENERIC DEFINITIONS AND THEOREMS *)
+Definition P_bircont_def:
+  P_bircont envtyl bpre ((SymbConcSt pc st status):(bir_programcounter_t, string, bir_val_t, bir_status_t) symb_concst_t) =
       (status = BST_Running /\
-       pc.bpc_index = 0 /\
-       bir_envty_list incr_birenvtyl st /\
-       bir_eval_exp (^bprecond x) (BEnv st) = SOME bir_val_true)
+       pc.bpc_index = 0 /\ (* TODO: comment here why do we need this? *)
+       bir_envty_list envtyl st /\
+       bir_eval_exp bpre (BEnv st) = SOME bir_val_true)
 End
 
-(* translate the property to BIR state property *)
-
-Theorem bprog_P_thm:
-  !x bs.
-  bprog_P x (birs_symb_to_concst bs) =
-      (bs.bst_status = BST_Running /\
-       bs.bst_pc.bpc_index = 0 /\
-       bir_envty_list_b incr_birenvtyl bs.bst_environ /\
-       bir_eval_exp (^bprecond x) bs.bst_environ = SOME bir_val_true)
-Proof
- REPEAT STRIP_TAC >>
-  FULL_SIMP_TAC (std_ss) [birs_symb_to_concst_def, bprog_P_def, bir_envty_list_b_thm, bir_BEnv_lookup_EQ_thm]
-QED
-
-Definition bprog_Q_def:
-  bprog_Q x
+Definition Q_bircont_def:
+  Q_bircont end_lbl vars Q
      ((SymbConcSt pc1 st1 status1):(bir_programcounter_t, string, bir_val_t, bir_status_t) symb_concst_t)
      ((SymbConcSt pc2 st2 status2):(bir_programcounter_t, string, bir_val_t, bir_status_t) symb_concst_t)
     =
      (
-       (pc2 = ^birs_state_end_lbl)
+       (pc2 = end_lbl)
        /\
        (status2 = BST_Running)
        /\
-       (bir_env_vars_are_initialised (BEnv st2) (set incr_prog_vars)) /\
-       (st2 "x10" = SOME (BVal_Imm (Imm64 (x + 1w))))
+       (bir_env_vars_are_initialised (BEnv st2) (vars)) /\
+       (Q (BEnv st2))
      )
 End
 
-Theorem bprog_Q_thm:
-  !x bs1 bs2.
-  bprog_Q x (birs_symb_to_concst bs1) (birs_symb_to_concst bs2) =
+(* translate the property to BIR state property *)
+
+Theorem P_bircont_thm:
+  !envtyl bpre bs.
+  P_bircont envtyl bpre (birs_symb_to_concst bs) =
+      (bs.bst_status = BST_Running /\
+       bs.bst_pc.bpc_index = 0 /\
+       bir_envty_list_b envtyl bs.bst_environ /\
+       bir_eval_exp bpre bs.bst_environ = SOME bir_val_true)
+Proof
+  REPEAT STRIP_TAC >>
+  FULL_SIMP_TAC (std_ss) [birs_symb_to_concst_def, P_bircont_def, bir_envty_list_b_thm, bir_BEnv_lookup_EQ_thm]
+QED
+
+Theorem Q_bircont_thm:
+  !end_lbl vars Q bs1 bs2.
+  Q_bircont end_lbl vars Q (birs_symb_to_concst bs1) (birs_symb_to_concst bs2) =
     (
-      (bs2.bst_pc = ^birs_state_end_lbl)
+      (bs2.bst_pc = end_lbl)
       /\
       (bs2.bst_status = BST_Running)
       /\
-      (bir_env_vars_are_initialised bs2.bst_environ (bir_vars_of_program ^bprog_tm))
+      (bir_env_vars_are_initialised bs2.bst_environ (vars))
       /\
-      (bir_env_lookup "x10" bs2.bst_environ = SOME (BVal_Imm (Imm64 (x + 1w))))
+      (Q bs2.bst_environ)
     )
 Proof
-FULL_SIMP_TAC (std_ss) [birs_symb_to_concst_def, bprog_Q_def, bir_envty_list_b_thm, incr_prog_vars_thm, birs_auxTheory.bir_BEnv_lookup_EQ_thm]
+  FULL_SIMP_TAC (std_ss) [birs_symb_to_concst_def, Q_bircont_def, bir_BEnv_lookup_EQ_thm]
 QED
-(* ........................... *)
 
-(* P is generic enough *)
 
-Theorem bprog_P_entails_thm:
-  P_entails_an_interpret (bir_symb_rec_sbir ^bprog_tm) (bprog_P pre_x10) (birs_symb_to_symbst ^birs_state_init_pre)
+
+Definition birs_state_init_pre_GEN_def:
+  birs_state_init_pre_GEN start_lbl birenvtyl bsysprecond =
+    <|
+      bsst_pc       := start_lbl;
+      bsst_environ  := bir_senv_GEN_list birenvtyl;
+      bsst_status   := BST_Running;
+      bsst_pcond    := bsysprecond
+    |>
+End
+
+Definition mk_bsysprecond_def:
+  mk_bsysprecond bpre envtyl = FST (THE (birs_eval_exp bpre (bir_senv_GEN_list envtyl)))
+End
+
+Theorem bir_envty_includes_birs_envty_of_senv_bir_senv_GEN_list_thm:
+  !envtyl.
+  (ALL_DISTINCT (MAP FST envtyl)) ==>
+  (bir_envty_includes_vs (birs_envty_of_senv (bir_senv_GEN_list envtyl)) (set (MAP PairToBVar envtyl)))
 Proof
-FULL_SIMP_TAC (std_ss++birs_state_ss) [P_entails_an_interpret_def] >>
+  REWRITE_TAC [bir_envTheory.bir_envty_includes_vs_def, bir_envTheory.bir_envty_includes_v_def, birs_envty_of_senv_def] >>
+  REPEAT STRIP_TAC >>
+  Cases_on `v` >>
+  FULL_SIMP_TAC (std_ss++holBACore_ss) [listTheory.MEM_MAP] >>
+  Cases_on `y` >>
+  FULL_SIMP_TAC (std_ss++holBACore_ss) [PairToBVar_def] >>
+  IMP_RES_TAC birs_auxTheory.bir_senv_GEN_list_APPLY_thm >>
+  FULL_SIMP_TAC (std_ss++holBACore_ss) [bir_senv_GEN_bvar_def]
+QED
+
+Theorem mk_bsysprecond_thm:
+  !bpre envtyl ty.
+  (ALL_DISTINCT (MAP FST envtyl)) ==>
+  (bir_vars_of_exp bpre SUBSET set (MAP PairToBVar envtyl)) ==>
+  (type_of_bir_exp bpre = SOME ty) ==>
+  (birs_eval_exp bpre (bir_senv_GEN_list envtyl) = SOME (mk_bsysprecond bpre envtyl,ty))
+Proof
+  REPEAT STRIP_TAC >>
+  `bir_envty_includes_vs (birs_envty_of_senv (bir_senv_GEN_list envtyl)) (bir_vars_of_exp bpre)` by (
+    METIS_TAC [bir_envty_includes_birs_envty_of_senv_bir_senv_GEN_list_thm, bir_envTheory.bir_envty_includes_vs_SUBSET]
+  ) >>
+  IMP_RES_TAC bir_symbTheory.birs_eval_exp_SOME_EQ_bir_exp_env_type_thm >>
+  ASM_SIMP_TAC std_ss [mk_bsysprecond_def]
+QED
+
+Theorem P_bircont_entails_thm:
+  !p envtyl bpre bsyspre start_lbl.
+  (bir_vars_of_program p = set (MAP PairToBVar envtyl)) ==>
+  (bir_vars_of_exp bpre SUBSET set (MAP PairToBVar envtyl)) ==>
+  (ALL_DISTINCT (MAP FST envtyl)) ==>
+  (IS_SOME (type_of_bir_exp bpre)) ==>
+  (bsyspre = mk_bsysprecond bpre envtyl) ==>
+  (P_entails_an_interpret
+    (bir_symb_rec_sbir p)
+    (P_bircont envtyl bpre)
+    (birs_symb_to_symbst (birs_state_init_pre_GEN start_lbl envtyl bsyspre)))
+Proof
+  FULL_SIMP_TAC (std_ss++birs_state_ss) [P_entails_an_interpret_def] >>
   REPEAT STRIP_TAC >>
 
   ASSUME_TAC ((GSYM o Q.SPEC `s`) birs_symb_to_concst_EXISTS_thm) >>
   FULL_SIMP_TAC (std_ss++birs_state_ss) [birs_symb_matchstate_EQ_thm] >>
 
-  FULL_SIMP_TAC (std_ss++birs_state_ss) [birs_symb_to_symbst_def, symb_symbst_pc_def] >>
+  FULL_SIMP_TAC (std_ss++birs_state_ss) [birs_symb_to_symbst_def, symb_symbst_pc_def, birs_state_init_pre_GEN_def] >>
 
   Cases_on `s` >> Cases_on `st` >>
-  FULL_SIMP_TAC (std_ss++holBACore_ss++symb_typesLib.symb_TYPES_ss) [bprog_P_def, birs_symb_to_concst_def, symb_concst_pc_def] >>
+  FULL_SIMP_TAC (std_ss++holBACore_ss++symb_typesLib.symb_TYPES_ss) [P_bircont_def, birs_symb_to_concst_def, symb_concst_pc_def, bir_BEnv_lookup_EQ_thm] >>
 
   Cases_on `b0` >>
-  FULL_SIMP_TAC (std_ss) [bir_envTheory.bir_env_lookup_def] >>
-  PAT_X_ASSUM ``A = (\B. C)`` (ASSUME_TAC o GSYM) >>
-  FULL_SIMP_TAC (std_ss) [boolTheory.ETA_THM] >>
+  FULL_SIMP_TAC (std_ss) [bir_env_lookup_I_thm] >>
 
-  `(ALL_DISTINCT (MAP FST incr_birenvtyl))` by EVAL_TAC >>
+  `?ty. birs_eval_exp bpre (bir_senv_GEN_list envtyl) = SOME (mk_bsysprecond bpre envtyl,ty)` by (
+    METIS_TAC [mk_bsysprecond_thm, optionTheory.IS_SOME_EXISTS]
+  ) >>
 
-  METIS_TAC [bprog_P_entails_gen_thm, birenvtyl_EVAL_thm, bprecond_birs_eval_exp_thm2]
+  METIS_TAC [bprog_P_entails_gen_thm]
 QED
 
-(* ........................... *)
-
-(* TODO: MOVE AWAY !!!!! GENERIC THEOREM *)
 Theorem birs_env_vars_are_initialised_IMP_thm:
   !H symbs senv env vs.
     birs_interpr_welltyped H ==>
@@ -292,83 +314,194 @@ Proof
   FULL_SIMP_TAC std_ss []
 QED
 
-Theorem birs_matchenv_gen_env_env_vars_are_initialised_incr_thm:
-  !H env x vs.
-     birs_interpr_welltyped H
-  ==>
-        birs_matchenv H
-          (birs_gen_env
-             [("x10",
-               BExp_BinExp BIExp_Plus
-                 (BExp_Den (BVar "sy_x10" (BType_Imm Bit64)))
-                 (BExp_Const (Imm64 1w)));
-              ("x1",BExp_Den (BVar "sy_x1" (BType_Imm Bit64)))])
-          env
-  ==>
-     symb_interpr_for_symbs
-          (birs_symb_symbols
-             <|bsst_pc :=
-                 <|bpc_label := BL_Address (Imm64 4w); bpc_index := 0|>;
-               bsst_environ :=
-                 birs_gen_env
-                   [("x10",
-                     BExp_BinExp BIExp_Plus
-                       (BExp_Den (BVar "sy_x10" (BType_Imm Bit64)))
-                       (BExp_Const (Imm64 1w)));
-                    ("x1",BExp_Den (BVar "sy_x1" (BType_Imm Bit64)))];
-               bsst_status := BST_Running;
-               bsst_pcond :=
-                 BExp_BinPred BIExp_Equal
-                   (BExp_Den (BVar "sy_x10" (BType_Imm Bit64)))
-                   (BExp_Const (Imm64 x))|>) H
- ==>
-    (vs = bir_vars_of_program ^bprog_tm) ==>
-          bir_env_vars_are_initialised env vs
+
+
+
+
+val birs_state_init_pre = ``birs_state_init_pre_GEN ^birs_state_init_lbl incr_birenvtyl (mk_bsysprecond (bir_incr_pre pre_x10) incr_birenvtyl)``;
+
+val incr_bsysprecond_thm = (computeLib.RESTR_EVAL_CONV [``birs_eval_exp``] THENC birs_stepLib.birs_eval_exp_CONV) ``mk_bsysprecond (bir_incr_pre pre_x10) incr_birenvtyl``;
+
+Theorem birs_state_init_pre_EQ_thm:
+  ^((snd o dest_comb) sys_i) = ^birs_state_init_pre
 Proof
-  REPEAT STRIP_TAC >>
-
-  IMP_RES_TAC birs_env_vars_are_initialised_IMP_thm >>
-  PAT_X_ASSUM ``!x. A`` (ASSUME_TAC o Q.SPEC `vs`) >>
-  POP_ASSUM (MATCH_MP_TAC) >>
-
-  (* cleanup proof state *)
-  ASM_REWRITE_TAC [] >>
-  REPEAT (POP_ASSUM (K ALL_TAC)) >>
-
-  (* concretize and normalize *)
-  FULL_SIMP_TAC (std_ss++birs_state_ss) [birs_symb_symbols_thm, birs_auxTheory.birs_exps_of_senv_thm] >>
-  FULL_SIMP_TAC (std_ss++holBACore_ss++listSimps.LIST_ss) [birs_gen_env_def, birs_gen_env_fun_def, birs_gen_env_fun_def, bir_envTheory.bir_env_lookup_def] >>
-  FULL_SIMP_TAC (std_ss++holBACore_ss++listSimps.LIST_ss) [birs_auxTheory.birs_exps_of_senv_COMP_thm] >>
-  CONV_TAC (RATOR_CONV (RAND_CONV (computeLib.RESTR_EVAL_CONV [``bir_vars_of_exp``] THENC SIMP_CONV (std_ss++holBACore_ss) [] THENC EVAL))) >>
-  CONV_TAC (RAND_CONV (SIMP_CONV (std_ss++listSimps.LIST_ss) [GSYM incr_prog_vars_thm, incr_prog_vars_def] THENC EVAL)) >>
-
-  (* finish the proof *)
-  REWRITE_TAC [birs_env_vars_are_initialised_INSERT_thm, birs_env_vars_are_initialised_EMPTY_thm, birs_env_var_is_initialised_def] >>
-  EVAL_TAC >>
-  SIMP_TAC (std_ss++holBACore_ss) [] >>
-  EVAL_TAC
+  REWRITE_TAC [birs_state_init_pre_GEN_def, mk_bsysprecond_def, incr_bsysprecond_thm] >>
+  CONV_TAC (computeLib.RESTR_EVAL_CONV [``birs_eval_exp``] THENC birs_stepLib.birs_eval_exp_CONV)
 QED
 
-(*
-Theorem bir_env_read_x10_lookup_thm:
-  !env x.
-  (bir_env_lookup "x10" env = SOME (BVal_Imm (Imm64 x))) ==>
-  (bir_env_read (BVar "x10" (BType_Imm Bit64)) env = SOME (BVal_Imm (Imm64 x)))
-Proof
-Cases_on `env` >>
+val incr_analysis_thm =
+  REWRITE_RULE [birs_state_init_pre_EQ_thm, GSYM bir_incr_prog_def] incr_symb_analysis_thm;
 
-  FULL_SIMP_TAC std_ss [bir_envTheory.bir_env_read_def, bir_envTheory.bir_env_check_type_def, bir_envTheory.bir_env_lookup_type_def, bir_envTheory.bir_env_lookup_def] >>
-  FULL_SIMP_TAC (std_ss++holBACore_ss) []
-QED
+Theorem incr_birenvtyl_EVAL_thm =
+ (REWRITE_CONV [incr_birenvtyl_def,
+   bir_lifting_machinesTheory.riscv_bmr_vars_EVAL,
+   bir_lifting_machinesTheory.riscv_bmr_temp_vars_EVAL] THENC EVAL)
+ ``incr_birenvtyl``;
+
+val birs_state_thm = REWRITE_CONV [incr_birenvtyl_EVAL_thm] birs_state_init_pre;
+
+(* ------ *)
+
+(* now the transfer *)
+
+val bprog_tm = (fst o dest_eq o concl) bir_incr_prog_def;
+
+val birs_symb_symbols_f_sound_prog_thm =
+  (SPEC (inst [Type`:'observation_type` |-> Type.alpha] bprog_tm) bir_symb_soundTheory.birs_symb_symbols_f_sound_thm);
+
+val birs_prop_transfer_thm =
+  (MATCH_MP symb_prop_transferTheory.symb_prop_transfer_thm birs_symb_symbols_f_sound_prog_thm);
+
+Definition bprog_P_def:
+  bprog_P x = P_bircont incr_birenvtyl (^bir_incr_pre x)
+End
+
+Definition bprog_Q_def:
+  bprog_Q x = Q_bircont (^birs_state_end_lbl) (set incr_prog_vars) (\env. bir_env_lookup "x10" env = SOME (BVal_Imm (Imm64 (x + 1w))))
+End
+(* ........................... *)
+
+(* P is generic enough *)
+(* taken from "bir_exp_to_wordsLib" *)
+val type_of_bir_exp_thms =
+    let
+      open bir_immTheory
+      open bir_valuesTheory
+      open bir_envTheory
+      open bir_exp_memTheory
+      open bir_bool_expTheory
+      open bir_extra_expsTheory
+      open bir_nzcv_expTheory
+      open bir_interval_expTheory
+      in [
+        type_of_bir_exp_def,
+        bir_var_type_def,
+        bir_type_is_Imm_def,
+        type_of_bir_imm_def,
+        BExp_Aligned_type_of,
+        BExp_unchanged_mem_interval_distinct_type_of,
+        bir_number_of_mem_splits_REWRS,
+        BType_Bool_def,
+        bir_exp_true_def,
+        bir_exp_false_def,
+        BExp_MSB_type_of,
+        BExp_nzcv_ADD_DEFS,
+        BExp_nzcv_SUB_DEFS,
+        n2bs_def,
+        BExp_word_bit_def,
+        BExp_Align_type_of,
+        BExp_ror_type_of,
+        BExp_LSB_type_of,
+        BExp_word_bit_exp_type_of,
+        BExp_ADD_WITH_CARRY_type_of,
+        BExp_word_reverse_type_of,
+        BExp_ror_exp_type_of
+      ] end;
+
+Theorem bprog_P_entails_thm[local]:
+  P_entails_an_interpret (bir_symb_rec_sbir ^bprog_tm) (bprog_P pre_x10) (birs_symb_to_symbst ^birs_state_init_pre)
+Proof
+  ASSUME_TAC (GSYM incr_prog_vars_thm) >>
+  `incr_prog_vars = MAP PairToBVar incr_birenvtyl` by (
+    SIMP_TAC std_ss [incr_birenvtyl_def, listTheory.MAP_MAP_o, PairToBVar_BVarToPair_I_thm, listTheory.MAP_ID]
+  ) >>
+  POP_ASSUM (fn thm => FULL_SIMP_TAC std_ss [thm]) >>
+  IMP_RES_TAC (SIMP_RULE std_ss [] P_bircont_entails_thm) >>
+
+  SIMP_TAC std_ss [bprog_P_def] >>
+  POP_ASSUM (ASSUME_TAC o Q.SPEC `bir_incr_pre pre_x10`) >>
+  `bir_vars_of_exp (bir_incr_pre pre_x10) SUBSET set (MAP PairToBVar incr_birenvtyl)` by (
+    PAT_X_ASSUM ``A = set B`` (fn thm => REWRITE_TAC [GSYM thm]) >>
+    SIMP_TAC (std_ss++holBACore_ss) [bir_incr_pre_def, bir_incr_pre_def] >>
+    SIMP_TAC (std_ss++pred_setLib.PRED_SET_ss) [GSYM incr_prog_vars_thm, incr_prog_vars_def, bir_incr_pre_def] >>
+    SIMP_TAC (std_ss++pred_setLib.PRED_SET_ss++holBACore_ss) [listTheory.MEM, pred_setTheory.IN_INSERT]
+  ) >>
+  POP_ASSUM (fn thm => FULL_SIMP_TAC std_ss [thm]) >>
+  `ALL_DISTINCT (MAP FST incr_birenvtyl)` by (
+    SIMP_TAC (std_ss++listSimps.LIST_ss) [incr_birenvtyl_EVAL_thm]
+  ) >>
+  POP_ASSUM (fn thm => FULL_SIMP_TAC std_ss [thm]) >>
+  `IS_SOME (type_of_bir_exp (bir_incr_pre pre_x10))` by (
+    SIMP_TAC std_ss [bir_incr_pre_def, bir_incr_pre_def] >>
+    CONV_TAC (RAND_CONV (SIMP_CONV (srw_ss()) type_of_bir_exp_thms)) >>
+    SIMP_TAC (std_ss++holBACore_ss) [optionTheory.option_CLAUSES]
+  ) >>
+  POP_ASSUM (fn thm => FULL_SIMP_TAC std_ss [thm])
+(*>>
+  POP_ASSUM (ASSUME_TAC o SPEC birs_state_init_lbl) >>
+
+  FULL_SIMP_TAC std_ss [mk_bsysprecond_def, GSYM bsysprecond_def] >>
+
+  FULL_SIMP_TAC std_ss [birs_state_init_pre_GEN_def]
 *)
+QED
+
+
+
+
+(* TODO: MOVE AWAY !!!!! GENERIC DEFINITIONS AND THEOREMS *)
+(*
+val varset_thm = incr_prog_vars_thm;
+*)
+fun Q_bircont_SOLVE3CONJS_TAC varset_thm = (
+    FULL_SIMP_TAC (std_ss) [Q_bircont_thm] >>
+    (* pc *)
+    CONJ_TAC >- (
+      REV_FULL_SIMP_TAC (std_ss++birs_state_ss) [birs_symb_matchstate_def]
+    ) >>
+    (* status Running *)
+    CONJ_TAC >- (
+      REV_FULL_SIMP_TAC (std_ss++birs_state_ss) [birs_symb_matchstate_def]
+    ) >>
+
+    (* bir_env_vars_are_initialised *)
+    CONJ_TAC >- (
+      PAT_X_ASSUM ``A = B`` (fn thm => FULL_SIMP_TAC std_ss [thm]) >>
+      PAT_X_ASSUM ``A = B`` (K ALL_TAC) >>
+      FULL_SIMP_TAC (std_ss++birs_state_ss) [birs_symb_matchstate_def, varset_thm] >>
+
+      IMP_RES_TAC birs_env_vars_are_initialised_IMP_thm >>
+      POP_ASSUM (K ALL_TAC) >>
+      PAT_X_ASSUM ``!x. A`` (ASSUME_TAC o SPEC ((snd o dest_eq o concl) varset_thm)) >>
+      POP_ASSUM (MATCH_MP_TAC) >>
+
+      (* cleanup proof state *)
+      REPEAT (POP_ASSUM (K ALL_TAC)) >>
+
+      (* concretize and normalize *)
+      FULL_SIMP_TAC (std_ss++birs_state_ss) [birs_symb_symbols_thm, birs_auxTheory.birs_exps_of_senv_thm] >>
+      FULL_SIMP_TAC (std_ss++holBACore_ss++listSimps.LIST_ss) [birs_gen_env_def, birs_gen_env_fun_def, birs_gen_env_fun_def, bir_envTheory.bir_env_lookup_def] >>
+      FULL_SIMP_TAC (std_ss++holBACore_ss++listSimps.LIST_ss) [birs_auxTheory.birs_exps_of_senv_COMP_thm] >>
+      CONV_TAC (RATOR_CONV (RAND_CONV (computeLib.RESTR_EVAL_CONV [``bir_vars_of_exp``] THENC SIMP_CONV (std_ss++holBACore_ss) [] THENC EVAL))) >>
+      (* TODO: improve this *)
+      CONV_TAC (RAND_CONV (computeLib.RESTR_EVAL_CONV [``bir_vars_of_program``] THENC SIMP_CONV (std_ss++HolBASimps.VARS_OF_PROG_ss++pred_setLib.PRED_SET_ss) [] THENC EVAL)) >>
+
+      (* finish the proof *)
+      REWRITE_TAC [birs_env_vars_are_initialised_INSERT_thm, birs_env_vars_are_initialised_EMPTY_thm, birs_env_var_is_initialised_def] >>
+      EVAL_TAC >>
+      SIMP_TAC (std_ss++holBACore_ss) [] >>
+      EVAL_TAC
+    )
+);
+
+
+
+
+(* ........................... *)
+(* proof for each end state individually: *)
+
+val sys1 = birs_state_init_pre;
+val (Pi_func, Pi_set) = dest_comb Pi_f;
+(* Pi_func should be exactly ``IMAGE birs_symb_to_symbst`` *)
+val sys2s = pred_setSyntax.strip_set Pi_set;
 
 (* FIXME: this is implicitly proven already in bir_envTheory.bir_env_read_def *)
 Theorem bir_eval_precond_lookup_pre_x10_incr_thm:
 !x env.
-  bir_eval_exp (bprecond x) env = SOME bir_val_true ==>
+  bir_eval_exp (bir_incr_pre x) env = SOME bir_val_true ==>
   bir_env_lookup "x10" env = SOME (BVal_Imm (Imm64 x))
 Proof
- rw [bprecond_def,bir_incr_pre_def] >>
+ rw [bir_incr_pre_def] >>
  Cases_on `env` >>
  FULL_SIMP_TAC (std_ss++holBACore_ss) [
   bir_envTheory.bir_env_lookup_type_def,
@@ -389,56 +522,34 @@ Proof
  FULL_SIMP_TAC (std_ss++holBACore_ss) []
 QED
 
-(* Q is implied by sys and Pi *)
-Theorem bprog_Pi_overapprox_Q_thm:
-  Pi_overapprox_Q (bir_symb_rec_sbir ^bprog_tm) (bprog_P pre_x10) (birs_symb_to_symbst ^birs_state_init_pre) ^Pi_f(*(IMAGE birs_symb_to_symbst {a;b;c;d})*) (bprog_Q pre_x10)
-Proof
-  REWRITE_TAC [bir_prop_transferTheory.bir_Pi_overapprox_Q_thm] >>
-  REPEAT GEN_TAC >>
-
-  REWRITE_TAC [pred_setTheory.IMAGE_INSERT, pred_setTheory.IMAGE_EMPTY, pred_setTheory.IN_INSERT, pred_setTheory.NOT_IN_EMPTY] >>
-  STRIP_TAC >> (
-    POP_ASSUM (fn thm => (ASSUME_TAC thm >> Q.ABBREV_TAC `sys3 = ^((snd o dest_eq o concl) thm)`)) >>
-    ASM_SIMP_TAC std_ss [] >>
-    rename1 `sys4 = sys3` >>
-    rename1 `sys4 = sys2` >>
-    PAT_X_ASSUM ``A = B`` (K ALL_TAC) >>
-
-    DISCH_TAC >>
-    POP_ASSUM (fn thm => (ASSUME_TAC thm >> Q.ABBREV_TAC `sys1 = ^((snd o dest_comb o fst o dest_comb o fst o dest_comb o concl) thm)`)) >>
-    POP_ASSUM (fn thm0 => POP_ASSUM (fn thm1 => (ASSUME_TAC thm0 >> ASSUME_TAC thm1))) >>
+(*
+val sys2 = hd sys2s;
+*)
+val Pi_thms = List.map (fn sys2 =>
+  prove(``
+    sys1 = ^sys1 ==>
+    sys2 = ^sys2 ==>
+    birs_symb_matchstate sys1 H bs ==>
+    bprog_P pre_x10 (birs_symb_to_concst bs) ==>
+    symb_interpr_ext H' H ==>
+    birs_symb_matchstate sys2 H' bs' ==>
+    bprog_Q pre_x10 (birs_symb_to_concst bs) (birs_symb_to_concst bs')
+  ``,
+    REWRITE_TAC [bprog_P_def, bprog_Q_def] >>
     REPEAT STRIP_TAC >>
+    Q_bircont_SOLVE3CONJS_TAC incr_prog_vars_thm >>
 
-    (* now the proof state is somewhat clean *)
-
-    FULL_SIMP_TAC (std_ss) [bprog_Q_thm] >>
-    (* pc *)
-    CONJ_TAC >- (
-      Q.UNABBREV_TAC `sys2` >>
-      FULL_SIMP_TAC (std_ss++birs_state_ss) [birs_symb_matchstate_def]
-    ) >>
-    (* status Running *)
-    CONJ_TAC >- (
-      Q.UNABBREV_TAC `sys2` >>
-      FULL_SIMP_TAC (std_ss++birs_state_ss) [birs_symb_matchstate_def]
-    ) >>
-
-    (* bir_env_vars_are_initialised *)
-    CONJ_TAC >- (
-      Q.UNABBREV_TAC `sys2` >>
-      FULL_SIMP_TAC (std_ss++birs_state_ss) [birs_symb_matchstate_def] >>
-      METIS_TAC [birs_matchenv_gen_env_env_vars_are_initialised_incr_thm]
-    ) >>
-
+    (* TODO: this is still hard coded for the example *)
     (* the property (here: pre_x10 + 1) *)
     `BVar "sy_x10" (BType_Imm Bit64) IN symb_interpr_dom H` by (
       `symb_interpr_for_symbs (birs_symb_symbols sys1) H` by (
         FULL_SIMP_TAC (std_ss++birs_state_ss) [birs_symb_matchstate_def]
       ) >>
 
-      Q.UNABBREV_TAC `sys1` >>
+      PAT_X_ASSUM ``A = ^sys1`` (fn thm => FULL_SIMP_TAC std_ss [thm]) >>
       POP_ASSUM (ASSUME_TAC o CONV_RULE (
-          REWRITE_CONV [bsysprecond_thm, birenvtyl_EVAL_thm] THENC
+          REWRITE_CONV [birs_state_init_pre_GEN_def, incr_bsysprecond_thm] THENC
+          REWRITE_CONV [birenvtyl_EVAL_thm] THENC
           computeLib.RESTR_EVAL_CONV [``birs_symb_symbols``] THENC
           aux_setLib.birs_symb_symbols_MATCH_CONV)
         ) >>
@@ -450,9 +561,10 @@ Proof
         FULL_SIMP_TAC (std_ss++birs_state_ss) [birs_symb_matchstate_def]
       ) >>
 
-      Q.UNABBREV_TAC `sys2` >>
+      PAT_X_ASSUM ``A = ^sys2`` (fn thm => FULL_SIMP_TAC std_ss [thm]) >>
       POP_ASSUM (ASSUME_TAC o CONV_RULE (
-          REWRITE_CONV [bsysprecond_thm, birenvtyl_EVAL_thm] THENC
+          REWRITE_CONV [birs_state_init_pre_GEN_def, incr_bsysprecond_thm] THENC
+          REWRITE_CONV [birenvtyl_EVAL_thm] THENC
           computeLib.RESTR_EVAL_CONV [``birs_symb_symbols``] THENC
           aux_setLib.birs_symb_symbols_MATCH_CONV)
         ) >>
@@ -464,19 +576,20 @@ Proof
       FULL_SIMP_TAC std_ss [symb_interpr_ext_def, symb_interprs_eq_for_def]
     ) >>
 
-    `bir_eval_exp (bprecond pre_x10) bs.bst_environ = SOME bir_val_true` by (
-      Q.UNABBREV_TAC `sys1` >>
-      FULL_SIMP_TAC (std_ss) [bprog_P_thm]
+    `bir_eval_exp (bir_incr_pre pre_x10) bs.bst_environ = SOME bir_val_true` by (
+      PAT_X_ASSUM ``A = ^sys1`` (fn thm => FULL_SIMP_TAC std_ss [thm]) >>
+      FULL_SIMP_TAC (std_ss) [P_bircont_thm]
     ) >>
 
     (* use bprog_P, but can also use the path condition in the end, or not? *)
     `symb_interpr_get H (BVar "sy_x10" (BType_Imm Bit64)) = SOME (BVal_Imm (Imm64 pre_x10))` by (
-      FULL_SIMP_TAC (std_ss) [bprog_P_thm] >>
+      FULL_SIMP_TAC (std_ss) [P_bircont_thm] >>
       `bir_env_lookup "x10" bs.bst_environ = SOME (BVal_Imm (Imm64 pre_x10))` by (
         METIS_TAC [bir_eval_precond_lookup_pre_x10_incr_thm]
       ) >>
 
-      Q.UNABBREV_TAC `sys1` >>
+
+      PAT_X_ASSUM ``A = ^sys1`` (fn thm => FULL_SIMP_TAC std_ss [thm]) >>
       FULL_SIMP_TAC (std_ss++birs_state_ss) [birs_symb_matchstate_def] >>
 
       FULL_SIMP_TAC (std_ss++birs_state_ss) [birs_matchenv_def, birs_interpret_fun_thm] >>
@@ -486,7 +599,7 @@ Proof
     ) >>
 
     (* now go through H' and sys2 with matchstate to show that the increment holds in bs' *)
-    Q.UNABBREV_TAC `sys2` >>
+    PAT_X_ASSUM ``A = ^sys2`` (fn thm => FULL_SIMP_TAC std_ss [thm]) >>
     FULL_SIMP_TAC (std_ss++birs_state_ss) [birs_symb_matchstate_def] >>
     REPEAT (PAT_X_ASSUM ``!A.B`` (ASSUME_TAC o EVAL_RULE o Q.SPEC `"x10"`)) >>
     FULL_SIMP_TAC (std_ss) [] >>
@@ -496,6 +609,22 @@ Proof
     FULL_SIMP_TAC (std_ss) [] >>
     REV_FULL_SIMP_TAC (std_ss) [birs_interpret_fun_ALT_def, birs_interpret_get_var_def] >>
     FULL_SIMP_TAC (std_ss++holBACore_ss) []
+  )
+) sys2s;
+
+(* ........................... *)
+
+(* Q is implied by sys and Pi *)
+Theorem bprog_Pi_overapprox_Q_thm[local]:
+  Pi_overapprox_Q (bir_symb_rec_sbir ^bprog_tm) (bprog_P pre_x10) (birs_symb_to_symbst ^birs_state_init_pre) ^Pi_f(*(IMAGE birs_symb_to_symbst {a;b;c;d})*) (bprog_Q pre_x10)
+Proof
+  REWRITE_TAC [bir_prop_transferTheory.bir_Pi_overapprox_Q_thm] >>
+  REPEAT GEN_TAC >>
+
+  REWRITE_TAC [pred_setTheory.IMAGE_INSERT, pred_setTheory.IMAGE_EMPTY, pred_setTheory.IN_INSERT, pred_setTheory.NOT_IN_EMPTY] >>
+  REPEAT STRIP_TAC >> (
+    FULL_SIMP_TAC std_ss [] >>
+    METIS_TAC Pi_thms
   )
 QED
 (* ........................... *)
@@ -513,7 +642,7 @@ val bprog_prop_holds_thm =
 (* lift to concrete state property *)
 val bprog_concst_prop_thm =
   SIMP_RULE (std_ss++birs_state_ss)
-    [birs_symb_symbst_pc_thm]
+    [birs_state_init_pre_GEN_def, birs_symb_symbst_pc_thm]
     (REWRITE_RULE
       [symb_prop_transferTheory.prop_holds_def]
       bprog_prop_holds_thm);
@@ -569,7 +698,7 @@ QED
 
 (* finish translation to pure BIR property *)
 Theorem bprog_bir_prop_thm = REWRITE_RULE
-    [bprog_P_thm, bprecond_def, bprog_Q_thm, birs_symb_concst_pc_thm, combinTheory.o_DEF, GSYM bir_programTheory.bir_exec_step_state_def, GSYM incr_analysis_L_def]
+    [bprog_P_def, P_bircont_thm, bir_incr_pre_def, bprog_Q_def, Q_bircont_thm, birs_symb_concst_pc_thm, combinTheory.o_DEF, GSYM bir_programTheory.bir_exec_step_state_def, GSYM incr_analysis_L_def]
     (REWRITE_RULE
       []
       bprog_to_concst_prop_thm)
@@ -584,7 +713,7 @@ val bir_frag_l_exit_tm = ``<|bpc_label := BL_Address (Imm64 ^bir_frag_l_exit_ml_
 
 Definition pre_bir_def:
   pre_bir x bs =
-       (bir_eval_exp (bprecond x) bs.bst_environ = SOME bir_val_true)
+       (bir_eval_exp (bir_incr_pre x) bs.bst_environ = SOME bir_val_true)
 End
 
 Definition post_bir_def:
@@ -621,8 +750,8 @@ Theorem bir_step_n_in_L_jgmt_thm[local]:
   (pre_bir_nL pre_x10)
   (post_bir_nL pre_x10)
 Proof
-REWRITE_TAC [bir_step_n_in_L_jgmt_def] >>
-  REWRITE_TAC [pre_bir_nL_def, pre_bir_def, bprecond_def] >>
+  REWRITE_TAC [bir_step_n_in_L_jgmt_def] >>
+  REWRITE_TAC [pre_bir_nL_def, pre_bir_def, bir_incr_pre_def] >>
   REPEAT STRIP_TAC >>
 
   ASSUME_TAC (Q.SPEC `st` bprog_bir_prop_thm) >>
@@ -766,7 +895,7 @@ Proof
     METIS_TAC [bir_vars_EQ_state_restrict_vars_THM]
   ) >>
 
-  FULL_SIMP_TAC std_ss [pre_bir_nL_def, pre_bir_def, bprecond_def, bir_exec_to_labels_triple_precond_def] >>
+  FULL_SIMP_TAC std_ss [pre_bir_nL_def, pre_bir_def, bir_exec_to_labels_triple_precond_def] >>
   METIS_TAC [bir_incr_pre_EQ_FOR_VARS_thm, bir_program_varsTheory.bir_state_EQ_FOR_VARS_ALT_DEF]
 QED
 
